spec/crypto/falcon.s.dfy
@@ -1,23 +1,22 @@
 include "mq_poly.s.dfy"
-include "mq_poly.i.dfy"
 include "mq_norm.s.dfy"
 
-abstract module falcon_s(CMQ: ntt_param_s, MQP: mq_poly_s(CMQ)) {
-    import MQN = mq_norm_s(CMQ)
+abstract module falcon_s(MQ: ntt_param_s, MQP: mq_poly_s(MQ)) {
+    import MQN = mq_norm_s(MQ)
 
-	type elem = CMQ.elem
+	type elem = MQ.elem
+    type n_elems = MQ.n_elems
     type nelem = MQN.nelem
-	type n_elems = CMQ.n_elems
 
-	// const Q := CMQ.Q;
-	const N := CMQ.N; 
+    const Q := MQ.Q;
+	const N := MQ.N; 
 
     function bound(): nat
 
     predicate falcon_verify(c0: seq<elem>, s2: seq<nelem>, h: seq<elem>)
         requires |c0| == |s2| == |h| == N.full;
     {
-        var tt0 := MQN.denormalize_nelems(s2);
+        var tt0 := MQN.denormalize_n_elems(s2);
         var tt1 := MQP.poly_mod(MQP.poly_mul(tt0, h), MQP.n_ideal());
         var tt2 := MQP.poly_sub(tt1, c0);
         var s1 := MQN.normalize_elems(tt2);
@@ -25,10 +24,3 @@ abstract module falcon_s(CMQ: ntt_param_s, MQP: mq_poly_s(CMQ)) {
     }
 }
 
-module falcon_512_i refines
-    falcon_s(ntt512_param_i, mq_poly_i(ntt512_param_i))
-{
-    function bound(): nat {
-        0x29845d6
-    }
-}
